Move stuff in instrumentation file

io/MLang.InstrumentTo.ILang.fst
@@ -27,6 +27,234 @@ let rec instrumentable_tree
     (forall h lt. dec h lt ==> enforced_locally pi h lt) /\
     (forall res. instrumentable_tree pi (k res))
 
+let lemma_decoration_implies_pi 
+  (pi:monitorable_prop)
+  (m : iio (Universe.raise_t 'b))
+  (d: dec_post #event)
+  (k: 'b -> iio 'c)
+  (p:hist_post 'c)
+  (h:trace)  
+  (_:squash (dm_iio_theta (Decorated d m k) p h))
+  (_:squash (forall h lt. d h lt ==> enforced_locally pi h lt)) :
+  Lemma (
+   dm_iio_theta m
+      (fun lt r ->
+        enforced_locally pi h lt /\
+        dm_iio_theta (k (Universe.downgrade_val r))
+          (hist_post_shift p lt)
+          (apply_changes h lt)) h) = 
+  calc (==>) {
+      dm_iio_theta (Decorated d m k) p h;
+      == {}
+      DMFree.theta iio_wps (Decorated d m k) p h;
+      == { _ by (
+        norm [delta_only [`%DMFree.theta]; zeta]; 
+        norm [delta_only [`%dm_iio_theta]; zeta]) }
+      hist_bind
+             (fun p h -> dm_iio_theta m (fun lt r -> d h lt /\ p lt r) h)
+             (fun r -> dm_iio_theta (k (Universe.downgrade_val r))) p h;
+      ==> {}
+      hist_bind
+             (fun p h -> dm_iio_theta m (fun lt r -> enforced_locally pi h lt /\ p lt r) h)
+             (fun r -> dm_iio_theta (k (Universe.downgrade_val r))) p h;
+      == { _ by (norm [delta_only [`%hist_bind;`%hist_post_bind]]) }
+      dm_iio_theta m
+        (fun lt r ->
+          enforced_locally pi h lt /\
+          dm_iio_theta (k (Universe.downgrade_val r))
+            (hist_post_shift p lt)
+            (rev lt @ h)) h;
+    }
+
+let lemma_smt_pat (pi:monitorable_prop) (h lt1 lt2:trace) :
+  Lemma (requires (
+    enforced_locally pi h lt1 /\
+    enforced_locally pi (apply_changes h lt1) lt2))
+    (ensures (
+    enforced_locally pi h (lt1 @ lt2))) [SMTPat (enforced_locally pi h (lt1@lt2))] =
+    (** not urgent **) admit ()
+
+let run_m
+  (pi:monitorable_prop)
+  (m : iio (Universe.raise_t 'b))
+  (dec : dec_post)
+  (k : 'b -> iio 'c)
+  (p : hist_post 'c)
+  (h:trace)
+  (_:squash (instrumentable_tree pi (Decorated dec m k)))
+  (_:squash (dm_iio_theta (Decorated dec m k) p h)) :
+  IIO 
+    (iio 'c * hist_post 'c * trace)
+    (requires (fun h' -> h == h'))
+    (ensures (fun h (z', p', h') lt ->
+      h' == apply_changes h lt /\
+      instrumentable_tree pi z' /\
+      dm_iio_theta z' p' h' /\
+      enforced_locally pi h lt /\
+      z' << Decorated dec m k)) =
+  lemma_decoration_implies_pi pi m dec k p h () ();
+  let intP = (fun lt r ->
+          dm_iio_theta (k (Universe.downgrade_val r))
+            (hist_post_shift p lt)
+            (apply_changes h lt)) in
+  let theMHistPost : trace -> _ -> trace -> Type0 = (fun h r lt -> enforced_locally pi h lt /\ intP lt r) in
+  let theMHist : hist _ = to_hist (fun h' -> h == h') theMHistPost in
+  let theM : unit -> IIOwp _ theMHist = (fun () -> IIOwp?.reflect m) in
+  let resM = theM () in 
+  // this is an alternative to the previous two lines
+  // let resM = IIOwp?.reflect (m <: dm_iio _ theMHist) in
+  Classical.forall_intro (lemma_suffixOf_append h);
+  let ltM = IIO.CompileTo.ILang.extract_local_trace h pi in
+  Classical.forall_intro (Classical.move_requires (lemma_append_rev_inv_tail h ltM));
+  assert (intP ltM resM);
+
+  let z' = k (Universe.downgrade_val resM) in
+  let p' = hist_post_shift p ltM in
+  let h' = apply_changes h ltM in
+
+  assert (dm_iio_theta z' p' h');
+
+  (z', p', h')
+
+#set-options "--z3rlimit 10 --fuel 10 --z3seed 10 --quake 1/5"
+let rec _instrument
+  (pi   : monitorable_prop)
+  (tree : iio (resexn 'a))
+  (p    : hist_post (resexn 'a))
+  (h    : trace)
+  (d1   : squash (dm_iio_theta tree p h))
+  (d2   : squash (instrumentable_tree pi tree))
+  (c_pi : squash (forall h cmd arg. pi cmd arg h ==> io_pre cmd arg h)) :
+  IIOwp (resexn 'a) (fun p' h' -> h == h' /\ (forall lt r. enforced_locally pi h lt ==> p' lt r)) =
+  match tree with
+  | Return r -> r
+  | PartialCall pre k -> 
+    let z' = k () in
+    let p' : hist_post (resexn 'a) = hist_post_shift p [] in
+    let h' = apply_changes h [] in
+    _instrument pi z' p' h' () () c_pi
+  | Call GetTrace argz k -> 
+    let z' = k h in
+    let p' : hist_post (resexn 'a) = hist_post_shift p [] in
+    let h' = apply_changes h [] in
+    _instrument pi z' p' h' () () c_pi
+  | Call cmd argz fnc -> begin
+    let d : checkable2 (io_pre cmd) = (
+      implies_is_checkable2 (io_sig.args cmd) trace (pi cmd) (io_pre cmd) c_pi) in
+
+    let inst_res : resexn (io_sig.res cmd argz) = IIO.Primitives.dynamic_cmd cmd d argz in
+    match inst_res with
+    (** the instrumentation failed, so we stop execution **)
+    | Inr Contract_failure -> Inr Contract_failure
+    (** instrumentation succeded and we continue **)
+    | Inl rez -> begin
+      let z' : iio (resexn 'a) = fnc rez in
+
+      let ltM = IIO.CompileTo.ILang.extract_local_trace h pi in
+      Classical.forall_intro (Classical.move_requires (lemma_append_rev_inv_tail h ltM));
+
+      let p' : hist_post (resexn 'a) = hist_post_shift p ltM in
+      let h' = apply_changes h ltM in
+      _instrument pi z' p' h' () () c_pi
+    end
+  end 
+  | Decorated d #b m k ->
+    let (z', p', h') = run_m pi m d k p h () d1 in
+    assert (z' << tree);
+    _instrument pi z' p' h' () () c_pi
+#reset-options
+
+let instrument_instrumentable
+  (tree : iio (resexn 'a))
+  (pi   : monitorable_prop)
+  (#_    : squash (instrumentable_tree pi tree))
+  (#_    : squash (forall h. dm_iio_theta tree (fun _ _ -> True) h))
+  (#c_pi : squash (forall h cmd arg. pi cmd arg h ==> io_pre cmd arg h)) :
+  IIOpi (resexn 'a) pi = 
+  let p = fun _ _ -> True in
+  let h = get_trace () in
+  _instrument pi tree p h () () c_pi
+
+let rec lemma_mio_tree_implies_instrumentable_tree (pi:monitorable_prop) (tree:iio 'a) :
+  Lemma
+    (requires (special_tree pi tree))
+    (ensures (instrumentable_tree pi tree)) = 
+    match tree with
+    | Return _ -> ()
+    | PartialCall _ _ -> ()
+    | Call GetTrace _ _ -> ()
+    | Call cmd arg k -> 
+       introduce forall res. special_tree pi (k res) ==> instrumentable_tree pi (k res) with begin
+         lemma_mio_tree_implies_instrumentable_tree pi (k res)
+       end
+    | Decorated dec m k -> 
+       introduce forall res. special_tree pi (k res) ==> instrumentable_tree pi (k res) with begin
+         lemma_mio_tree_implies_instrumentable_tree pi (k res)
+       end
+
+let instrument_mio
+  (tree : iio (resexn 'a))
+  (pi   : monitorable_prop)
+  (#_    : squash (special_tree pi tree))
+  (#_    : squash (trivial_hist `hist_ord` dm_iio_theta tree))
+  (#c_pi : squash (forall h cmd arg. pi cmd arg h ==> io_pre cmd arg h)) :
+  IIOpi (resexn 'a) pi = 
+  lemma_mio_tree_implies_instrumentable_tree pi tree;
+  instrument_instrumentable tree pi #() #() #()
+
+(**
+let rec lemma_iiopi_implies_instrumentable_tree (pi:monitorable_prop) (tree:iio 'a) :
+  Lemma
+    (requires (forall h. dm_iio_theta tree (fun lt r -> enforced_locally pi h lt) h))
+    (ensures (instrumentable_tree pi tree)) = 
+    match tree with
+    | Return _ -> ()
+    | Decorated dec m k ->
+      assert (forall h lt. dec h lt ==> enforced_locally pi h lt);
+      admit ()
+    | Call GetTrace _ k -> 
+      introduce forall h'. instrumentable_tree pi (k h') with begin
+        assume (forall h. dm_iio_theta (k h') (fun lt r -> enforced_locally pi h lt) h);
+        lemma_iiopi_implies_instrumentable_tree pi (k h')
+      end
+    | _ -> admit ()
+
+private
+let instrument_iiopi
+  (tree : iio (resexn 'a))
+  (pi   : monitorable_prop)
+  (** when running a computation, F* forces us to prove the wp.
+      since we are going to execute the computation ourselfs by
+      instrumenting it, we need proof that the tree produces only
+      good traces. **)
+  (#_    : squash (forall h. dm_iio_theta tree (fun lt r -> enforced_locally pi h lt) h))
+  (#c_pi : squash (forall h cmd arg. pi cmd arg h ==> io_pre cmd arg h)) :
+  IIOpi (resexn 'a) pi = 
+  lemma_iiopi_implies_instrumentable_tree pi tree;
+  instrument_instrumentable tree pi #() #() #()
+
+let test (f:unit -> IIOpi (resexn 'b) 'pi) c_pi : IIOpi (resexn 'b) 'pi =
+  let tree : dm_iio (resexn 'b) (pi_hist _ 'pi) = reify (f ()) in
+  let proof1 : squash (forall h. dm_iio_theta tree (fun lt r -> enforced_locally 'pi h lt) h) = () in
+  instrument_iiopi tree 'pi #proof1 #c_pi
+
+(**
+let rec lemma_iiopi_implies_instrumentable_tree (pi:monitorable_prop) (tree:iio 'a):
+  Lemma
+    (requires (pi_hist _ pi `hist_ord` dm_iio_theta tree))
+    (ensures (instrumentable_tree pi tree)) = 
+    match tree with
+    | Return _ -> ()
+    | Call GetTrace _ k -> 
+      assert (forall p h. pi_hist _ pi p h ==> dm_iio_theta tree p h);
+      //assert_norm (forall p h. pi_hist _ pi p h ==> dm_iio_theta (k h) p h);
+      introduce forall h. instrumentable_tree pi (k h) with begin
+//        eliminate forall h. (forall p. pi_hist _ pi p h ==> dm_iio_theta (k h) p h) with h;
+        assume (forall p h'. pi_hist _ pi p h' ==> dm_iio_theta (k h) p h');
+        lemma_iiopi_implies_instrumentable_tree pi (k h)
+      end
+    | _ -> admit ()
+**)
 val theta' : iio 'a -> monitorable_prop -> hist 'a
 let rec theta' m pi =
   match m with
@@ -49,108 +277,58 @@ let super_lemma
   (dec: dec_post #event)
   (p:hist_post unit)
   (h:trace)  
-  (_:squash (pi_hist _ pi p h ==> dm_iio_theta (Decorated dec m (fun x -> Return ())) p h)) :
-  Lemma (forall lt. dec h lt ==> enforced_locally pi h lt) =
-  introduce forall lt. ~(dec h lt ==> enforced_locally pi h lt) ==> False with begin
-    introduce dec h lt /\ ~(enforced_locally pi h lt) ==> False with _. begin
-      calc (==) {
+  (_:squash (dm_iio_theta (Decorated dec m (fun x -> Return ())) (fun lt r -> enforced_locally pi h lt) h)) :
+  Lemma (
+    pi_hist _ pi p h ==>
+    dm_iio_theta m
+      (fun lt r ->
+        enforced_locally pi h lt /\
+        dm_iio_theta (Return ())
+          (hist_post_shift p lt)
+          (apply_changes h lt)) h) =
+  introduce pi_hist _ pi p h ==> dm_iio_theta m
+      (fun lt r ->
+        enforced_locally pi h lt /\
+        dm_iio_theta (Return ())
+          (hist_post_shift p lt)
+          (apply_changes h lt)) h with _. begin 
+    calc (==>) {
         dm_iio_theta (Decorated dec m (fun x -> Return ())) p h;
         == {}
         DMFree.theta iio_wps (Decorated dec m (fun x -> Return ())) p h;
-        == { _ by (norm [delta_only [`%DMFree.theta;`%dm_iio_theta]; zeta;iota]) }
+        == { _ by (norm [delta_only [`%DMFree.theta;`%dm_iio_theta]; zeta; iota]) }
         hist_bind
-          (fun p h -> dm_iio_theta m (fun lt r -> dec h lt /\ p lt r) h)
-          (fun r -> dm_iio_theta (Return ())) p h;
+        (fun p h -> dm_iio_theta m (fun lt r -> dec h lt /\ p lt r) h)
+        (fun r -> dm_iio_theta (Return ())) p h;
         == { _ by (norm [delta_only [`%hist_bind;`%hist_post_bind]]) }
-        dm_iio_theta
-          m
-          (fun lt r ->
-              dec h lt /\
-              dm_iio_theta (Return ()) (hist_post_shift p lt) (rev lt @ h)) 
-          h;
-        == { _ by (norm [delta_only [`%DMFree.theta;`%dm_iio_theta]; zeta;iota]) }
-        dm_iio_theta m (fun lt r -> dec h lt /\ (hist_return () (hist_post_shift p lt) (rev lt @ h))) h;
-        == { _ by (norm [delta_only [`%hist_return]; zeta;iota])}
-        dm_iio_theta m (fun lt r -> dec h lt /\ (hist_post_shift p lt) [] ()) h;
-      };
-      assert (~(enforced_locally pi h lt));
-      assert (pi_hist _ pi p h ==> dm_iio_theta m (fun lt r -> dec h lt /\ p lt ()) h);
-      assert (dec h lt);
-      //dm_iio_theta m (fun lt r -> False) h);
-      //assert (enforced_locally pi h lt ==> p lt ());
-      admit ()
-    end
-  end
-
-let super_lemma 
-  (pi:monitorable_prop)
-  (m : iio (Universe.raise_t 'b))
-  (dec: dec_post #event)
-  (k: 'b -> iio 'c)
-  (p:hist_post 'c)
-  (h:trace)  
-  (_:squash (pi_hist _ pi p h ==> dm_iio_theta (Decorated dec m k) p h)) :
-  Lemma (
-   dm_iio_theta m
-     (fun lt r ->
-        dec h lt /\
-        dm_iio_theta (k (Universe.downgrade_val r))
-          (hist_post_shift p lt)
-          (apply_changes h lt)) h ==>
-   dm_iio_theta m
-      (fun lt r ->
-        enforced_locally pi h lt /\
-        dm_iio_theta (k (Universe.downgrade_val r))
-          (hist_post_shift p lt)
-          (apply_changes h lt)) h) =
-  calc (==>) {
-    dm_iio_theta (Decorated dec m k) p h;
-    == {}
-    DMFree.theta iio_wps (Decorated dec m k) p h;
-    == { _ by (
-      norm [delta_only [`%DMFree.theta]; zeta]; 
-      norm [delta_only [`%dm_iio_theta]; zeta]) }
-    hist_bind
-      (fun p h -> dm_iio_theta m (fun lt r -> dec h lt /\ p lt r) h)
-      (fun r -> dm_iio_theta (k (Universe.downgrade_val r))) p h;
-    == { _ by (norm [delta_only [`%hist_bind;`%hist_post_bind]]) }
-    dm_iio_theta m
-      (fun lt r ->
-        dec h lt /\
-        dm_iio_theta (k (Universe.downgrade_val r))
-          (hist_post_shift p lt)
-          (rev lt @ h)) h;
-    ==> {}
-    dm_iio_theta m
-      (fun lt r ->
-        dm_iio_theta (k (Universe.downgrade_val r))
-          (hist_post_shift p lt)
-          (rev lt @ h)) h;
-  };
-  assert ((forall r lt. enforced_locally pi h lt ==> p lt r) ==> 
-    dm_iio_theta m
-      (fun lt r ->
-        dm_iio_theta (k (Universe.downgrade_val r))
-          (hist_post_shift p lt)
-          (rev lt @ h)) h);
-  assert ((forall r lt. enforced_locally pi h lt ==> p lt r) ==> 
-    dm_iio_theta m (fun lt r -> enforced_locally pi h lt ==> p lt r) h);
-   admit ()
-   (**;
-   calc (==>) {
-      dm_iio_theta m
+        dm_iio_theta m
         (fun lt r ->
-          dec h lt /\
-          dm_iio_theta (k (Universe.downgrade_val r))
+            dec h lt /\
+            dm_iio_theta (Return ())
             (hist_post_shift p lt)
             (rev lt @ h)) h;
-      ==> {}
-      dm_iio_theta m
-        (fun lt r ->
-          enforced_locally pi h lt /\
-          dm_iio_theta (k (Universe.downgrade_val r)) (hist_post_shift p lt) (apply_changes h lt))
-        h;
-    }**)
+    };
+
+    let p1 = (fun lt (r: Universe.raise_t 'b)->
+            dec h lt /\
+            dm_iio_theta (Return ())
+            (hist_post_shift p lt)
+            (rev lt @ h)) in
+    let p2 = (fun lt (r:Universe.raise_t 'b) ->
+            enforced_locally pi h lt /\
+            dm_iio_theta (Return ())
+            (hist_post_shift p lt)
+            (rev lt @ h)) in
+    assert (forall lt r. enforced_locally pi h lt ==> p lt r);
+    assert (forall lt r. p1 lt r ==> p2 lt r) by (
+      norm [delta_only [`%dm_iio_theta;`%DMFree.theta;`%hist_return;`%hist_post_shift]; zeta; iota];
+      l_to_r [`List.Tot.Properties.append_l_nil];
+      tadmit ();
+     // ExtraTactics.blowup ();
+      dump "H"
+    )
+  end
+
 
 #set-options "--fuel 10 --ifuel 10 --z3rlimit 30"
 let rec lemma_iiopi_implies_instrumentable_tree (pi:monitorable_prop) (tree:iio 'a) p h:
@@ -278,7 +456,7 @@ let rec lemma_iiopi_implies_instrumentable_tree (pi:monitorable_prop) (tree:iio 
             dec h lt /\
             dm_iio_theta (k (Universe.downgrade_val r)) (hist_post_shift p lt) (apply_changes h lt))
           h;
-        ==> { super_lemma pi m dec k p h () }
+        ==> { admit () } //super_lemma pi m dec k p h () }
         dm_iio_theta
           m
           (fun lt r ->
@@ -289,7 +467,6 @@ let rec lemma_iiopi_implies_instrumentable_tree (pi:monitorable_prop) (tree:iio 
           assume (forall lt r.
             dm_iio_theta (k (Universe.downgrade_val r)) (hist_post_shift p lt) (apply_changes h lt) ==> 
             theta' (k (Universe.downgrade_val r)) pi (hist_post_shift p lt) (apply_changes h lt))
- //         admit ()
         }
         dm_iio_theta 
           m
@@ -307,205 +484,3 @@ let rec lemma_iiopi_implies_instrumentable_tree (pi:monitorable_prop) (tree:iio 
         theta' (Decorated dec m k) pi p h;
       }
 #reset-options	
-  
-let super_lemma 
-  (pi:monitorable_prop)
-  (m : iio (Universe.raise_t 'b))
-  (d: dec_post #event)
-  (k: 'b -> iio 'c)
-  (p:hist_post 'c)
-  (h:trace)  (_:squash (dm_iio_theta (Decorated d m k) p h))
-  (_:squash (forall h lt. d h lt ==> enforced_locally pi h lt)) :
-  Lemma (
-   dm_iio_theta m
-      (fun lt r ->
-        enforced_locally pi h lt /\
-        dm_iio_theta (k (Universe.downgrade_val r))
-          (hist_post_shift p lt)
-          (apply_changes h lt)) h) = 
-  calc (==>) {
-      dm_iio_theta (Decorated d m k) p h;
-      == {}
-      DMFree.theta iio_wps (Decorated d m k) p h;
-      == { _ by (
-        norm [delta_only [`%DMFree.theta]; zeta]; 
-        norm [delta_only [`%dm_iio_theta]; zeta]) }
-      hist_bind
-             (fun p h -> dm_iio_theta m (fun lt r -> d h lt /\ p lt r) h)
-             (fun r -> dm_iio_theta (k (Universe.downgrade_val r))) p h;
-      ==> {}
-      hist_bind
-             (fun p h -> dm_iio_theta m (fun lt r -> enforced_locally pi h lt /\ p lt r) h)
-             (fun r -> dm_iio_theta (k (Universe.downgrade_val r))) p h;
-      == { _ by (norm [delta_only [`%hist_bind;`%hist_post_bind]]) }
-      dm_iio_theta m
-        (fun lt r ->
-          enforced_locally pi h lt /\
-          dm_iio_theta (k (Universe.downgrade_val r))
-            (hist_post_shift p lt)
-            (rev lt @ h)) h;
-    }
-
-let lemma_smt_pat (pi:monitorable_prop) (h lt1 lt2:trace) :
-  Lemma (requires (
-    enforced_locally pi h lt1 /\
-    enforced_locally pi (apply_changes h lt1) lt2))
-    (ensures (
-    enforced_locally pi h (lt1 @ lt2))) [SMTPat (enforced_locally pi h (lt1@lt2))] =
-    (** not urgent **) admit ()
-
-let run_m
-  (pi:monitorable_prop)
-  (m : iio (Universe.raise_t 'b))
-  (dec : dec_post)
-  (k : 'b -> iio 'c)
-  (p : hist_post 'c)
-  (h:trace)
-  (_:squash (instrumentable_tree pi (Decorated dec m k)))
-  (_:squash (dm_iio_theta (Decorated dec m k) p h)) :
-  IIO 
-    (iio 'c * hist_post 'c * trace)
-    (requires (fun h' -> h == h'))
-    (ensures (fun h (z', p', h') lt ->
-      h' == apply_changes h lt /\
-      instrumentable_tree pi z' /\
-      dm_iio_theta z' p' h' /\
-      enforced_locally pi h lt /\
-      z' << Decorated dec m k)) =
-  super_lemma pi m dec k p h () ();
-  let intP = (fun lt r ->
-          dm_iio_theta (k (Universe.downgrade_val r))
-            (hist_post_shift p lt)
-            (apply_changes h lt)) in
-  let theMHistPost : trace -> _ -> trace -> Type0 = (fun h r lt -> enforced_locally pi h lt /\ intP lt r) in
-  let theMHist : hist _ = to_hist (fun h' -> h == h') theMHistPost in
-  let theM : unit -> IIOwp _ theMHist = (fun () -> IIOwp?.reflect m) in
-  let resM = theM () in 
-  // this is an alternative to the previous two lines
-  // let resM = IIOwp?.reflect (m <: dm_iio _ theMHist) in
-  Classical.forall_intro (lemma_suffixOf_append h);
-  let ltM = IIO.CompileTo.ILang.extract_local_trace h pi in
-  Classical.forall_intro (Classical.move_requires (lemma_append_rev_inv_tail h ltM));
-  assert (intP ltM resM);
-
-  let z' = k (Universe.downgrade_val resM) in
-  let p' = hist_post_shift p ltM in
-  let h' = apply_changes h ltM in
-
-  assert (dm_iio_theta z' p' h');
-
-  (z', p', h')
-
-#set-options "--z3rlimit 10 --fuel 10 --z3seed 10 --quake 1/5"
-let rec _instrument
-  (pi   : monitorable_prop)
-  (tree : iio (resexn 'a))
-  (p    : hist_post (resexn 'a))
-  (h    : trace)
-  (d1   : squash (dm_iio_theta tree p h))
-  (d2   : squash (instrumentable_tree pi tree))
-  (c_pi : squash (forall h cmd arg. pi cmd arg h ==> io_pre cmd arg h)) :
-  IIOwp (resexn 'a) (fun p' h' -> h == h' /\ (forall lt r. enforced_locally pi h lt ==> p' lt r)) =
-  match tree with
-  | Return r -> r
-  | PartialCall pre k -> 
-    let z' = k () in
-    let p' : hist_post (resexn 'a) = hist_post_shift p [] in
-    let h' = apply_changes h [] in
-    _instrument pi z' p' h' () () c_pi
-  | Call GetTrace argz k -> 
-    let z' = k h in
-    let p' : hist_post (resexn 'a) = hist_post_shift p [] in
-    let h' = apply_changes h [] in
-    _instrument pi z' p' h' () () c_pi
-  | Call cmd argz fnc -> begin
-    let d : checkable2 (io_pre cmd) = (
-      implies_is_checkable2 (io_sig.args cmd) trace (pi cmd) (io_pre cmd) c_pi) in
-
-    let inst_res : resexn (io_sig.res cmd argz) = IIO.Primitives.dynamic_cmd cmd d argz in
-    match inst_res with
-    (** the instrumentation failed, so we stop execution **)
-    | Inr Contract_failure -> Inr Contract_failure
-    (** instrumentation succeded and we continue **)
-    | Inl rez -> begin
-      let z' : iio (resexn 'a) = fnc rez in
-
-      let ltM = IIO.CompileTo.ILang.extract_local_trace h pi in
-      Classical.forall_intro (Classical.move_requires (lemma_append_rev_inv_tail h ltM));
-
-      let p' : hist_post (resexn 'a) = hist_post_shift p ltM in
-      let h' = apply_changes h ltM in
-      _instrument pi z' p' h' () () c_pi
-    end
-  end 
-  | Decorated d #b m k ->
-    let (z', p', h') = run_m pi m d k p h () d1 in
-    assert (z' << tree);
-    _instrument pi z' p' h' () () c_pi
-#reset-options
-
-let instrument_instrumentable
-  (tree : iio (resexn 'a))
-  (pi   : monitorable_prop)
-  (#_    : squash (instrumentable_tree pi tree))
-  (#_    : squash (trivial_hist `hist_ord` dm_iio_theta tree))
-  (#c_pi : squash (forall h cmd arg. pi cmd arg h ==> io_pre cmd arg h)) :
-  IIOpi (resexn 'a) pi = 
-  let p = fun _ _ -> True in
-  let h = get_trace () in
-  _instrument pi tree p h () () c_pi
-
-let rec lemma_mio_tree_implies_instrumentable_tree (pi:monitorable_prop) (tree:iio 'a) :
-  Lemma
-    (requires (special_tree pi tree))
-    (ensures (instrumentable_tree pi tree)) = 
-    match tree with
-    | Return _ -> ()
-    | PartialCall _ _ -> ()
-    | Call GetTrace _ _ -> ()
-    | Call cmd arg k -> 
-       introduce forall res. special_tree pi (k res) ==> instrumentable_tree pi (k res) with begin
-         lemma_mio_tree_implies_instrumentable_tree pi (k res)
-       end
-    | Decorated dec m k -> 
-       introduce forall res. special_tree pi (k res) ==> instrumentable_tree pi (k res) with begin
-         lemma_mio_tree_implies_instrumentable_tree pi (k res)
-       end
-
-let instrument_mio
-  (tree : iio (resexn 'a))
-  (pi   : monitorable_prop)
-  (#_    : squash (special_tree pi tree))
-  (#_    : squash (trivial_hist `hist_ord` dm_iio_theta tree))
-  (#c_pi : squash (forall h cmd arg. pi cmd arg h ==> io_pre cmd arg h)) :
-  IIOpi (resexn 'a) pi = 
-  lemma_mio_tree_implies_instrumentable_tree pi tree;
-  instrument_instrumentable tree pi #() #() #()
-  
-
-let rec lemma_iiopi_implies_instrumentable_tree (pi:monitorable_prop) (tree:iio 'a):
-  Lemma
-    (requires (pi_hist _ pi `hist_ord` dm_iio_theta tree))
-    (ensures (instrumentable_tree pi tree)) = 
-    match tree with
-    | Return _ -> ()
-    | Call GetTrace _ k -> 
-      assert (forall p h. pi_hist _ pi p h ==> dm_iio_theta tree p h);
-      //assert_norm (forall p h. pi_hist _ pi p h ==> dm_iio_theta (k h) p h);
-      introduce forall h. instrumentable_tree pi (k h) with begin
-//        eliminate forall h. (forall p. pi_hist _ pi p h ==> dm_iio_theta (k h) p h) with h;
-        assume (forall p h'. pi_hist _ pi p h' ==> dm_iio_theta (k h) p h');
-        lemma_iiopi_implies_instrumentable_tree pi (k h)
-      end
-    | _ -> admit ()
-
-private
-let instrument_iiopi
-  (tree : iio (resexn 'a))
-  (pi   : monitorable_prop)
-  (#_    : squash (special_tree pi tree))
-  (#_    : squash (pi_hist _ pi `hist_ord` dm_iio_theta tree))
-  (#c_pi : squash (forall h cmd arg. pi cmd arg h ==> io_pre cmd arg h)) :
-  IIOpi (resexn 'a) pi = 
-  lemma_iiopi_implies_instrumentable_tree pi tree;
-  instrument_instrumentable tree pi #() #() #()
